examples/opaque/game.v
@@ -8,7 +8,7 @@ From stdpp Require Import namespaces.
 From iris.algebra Require Import agree auth csum gset gmap excl frac.
 From iris.algebra Require Import max_prefix_list.
 From iris.heap_lang Require Import notation proofmode.
-From iris.heap_lang.lib Require Import lock ticket_lock.
+From iris.heap_lang.lib Require Import par lock ticket_lock.
 From cryptis.examples Require Import alist.
 
 From cryptis.examples.opaque Require Import impl server_proofs client_proofs shared.
@@ -20,7 +20,7 @@ Unset Printing Implicit Defensive.
 
 Section Game.
 
-Context `{!cryptisGS Σ, !heapGS Σ}.
+Context `{!cryptisGS Σ, !heapGS Σ, !spawnG Σ}.
 Notation iProp := (iProp Σ).
 
 Definition game : val :=
@@ -30,9 +30,14 @@ let: "uid" := mk_nonce #() in
 let: "pw" := mk_nonce #() in
 let: "db" := AList.new #() in
 AList.insert "db" "uid" (Server.make_file "pw") ;;
-Fork (Server.session "db" "c");;
-Client.session "uid" "c" "pw";;
-assert: (~ eq_term "pw" (recv "c")).
+let: "SKs" := Server.session "db" "c" ||| Client.session "uid" "c" "pw" in
+assert: (~ eq_term "pw" (recv "c")) ;;
+(bind: "SK" := (Fst "SKs") in
+   assert: (~ eq_term "SK" (recv "c"));;
+           NONE) ;;
+(bind: "SK" := (Snd "SKs") in
+   assert: (~ eq_term "SK" (recv "c"));;
+           NONE).
 
 Lemma wp_game :
 {{{ cryptis_ctx
@@ -41,7 +46,7 @@ Lemma wp_game :
 game #()
 {{{ x , RET x ; True }}}.
 Proof.
-iIntros "%ϕ (#Hcryptis & h_pred_tok & s_pred_tok) Hhl".
+iIntros "%ϕ (#? & h_pred_tok & s_pred_tok) Hhl".
 iMod (opaque_alloc with "h_pred_tok s_pred_tok") as
   "[(#? & #? & #? & #? & #? & #? & #?) _]" => //.
 wp_lam.
@@ -70,17 +75,21 @@ iApply (AList.wp_insert with "Halist").
 iNext.
 iIntros "Halist".
 wp_pures.
-wp_apply (wp_fork with "[Halist Hopaquefile]").
+wp_apply (wp_par SK_priv' SK_priv' with "[Halist Hopaquefile]").
 iApply (wp_server_session db c (<[uid:=file]> ∅)  with "[Halist Hopaquefile]") => //.
 do !iSplit => //.
 iApply big_sepM_insert => //.
-do !iSplit => //. auto.
-wp_pures.
-wp_bind (Client.session uid c pw).
+do !iSplit => //.
+iNext.
+iIntros "%x".
+by iApply SK_priv_eq.
 iApply (wp_client_session uid pw c).
 do !iSplit => //.
 iNext.
-iIntros "%_ _".
+iIntros "%_".
+by iApply SK_priv_eq.
+iIntros "%SK1 %SK2 [(%SK1' & -> & HprivSK1) (%SK2' & -> & HprivSK2)]".
+iNext.
 wp_pures.
 wp_apply wp_assert.
 wp_apply wp_recv => //.
@@ -92,8 +101,48 @@ iDestruct "Hprivpw" as "[Hprivpw _]".
 iDestruct ("Hprivpw" with "Hpubattack") as "Hcontra".
 all: wp_pures.
 by iDestruct "Hcontra" as "%Hcontra".
+clear H.
 iModIntro.
 iSplit => //.
+iNext.
+wp_pures.
+wp_bind (bind: _ := _ in _)%E.
+iApply (wp_wand _ _ _ (λ v, ⌜v = InjLV #() ⌝)%I with "[HprivSK1]").
+destruct SK1'; wp_pures => //.
+wp_apply wp_assert.
+wp_apply wp_recv => //.
+iIntros "%guess #pubguess".
+wp_bind (eq_term _ _).
+wp_eq_term H.
+rewrite H.
+iSpecialize ("HprivSK1" with "pubguess").
+wp_pures.
+by iDestruct "HprivSK1" as "%HprivSK1".
+wp_pures.
+iModIntro.
+iSplit => //.
+iNext.
+by wp_pures.
+iIntros "%_ ->".
+wp_pures.
+wp_bind (bind: _ := _ in _)%E.
+iApply (wp_wand _ _ _ (λ v, ⌜v = InjLV #() ⌝)%I with "[HprivSK2]").
+destruct SK2'; wp_pures => //.
+wp_apply wp_assert.
+wp_apply wp_recv => //.
+iIntros "%guess #pubguess".
+wp_bind (eq_term _ _).
+wp_eq_term H.
+rewrite H.
+iSpecialize ("HprivSK2" with "pubguess").
+wp_pures.
+by iDestruct "HprivSK2" as "%HprivSK2".
+wp_pures.
+iModIntro.
+iSplit => //.
+iNext.
+by wp_pures.
+iIntros "%_ ->".
 by iApply "Hhl".
 Qed.
 
